Add timeouts.

src/super/prover.lean
@@ -41,6 +41,7 @@ meta def run_prover_loop
   (clause_selection : clause_selection_strategy)
   (preprocessing_rules : list (prover unit))
   (inference_rules : list inference)
+  (max_iters : ℕ)
   : ℕ → prover (option expr) | i := do
 sequence' preprocessing_rules,
 new ← take_newly_derived, new.mmap' register_as_passive,
@@ -70,6 +71,7 @@ given ← literal_selection given,
   fmt ← pp given, trace (to_fmt "given: " ++ fmt)),
 add_active given,
 seq_inferences inference_rules given,
+when (i ≥ max_iters) $ fail "reached maximum number of iterations in saturation loop",
 run_prover_loop (i+1)
 
 meta def default_preprocessing : list (prover unit) :=
@@ -90,7 +92,12 @@ end super
 
 open super
 
-meta def super (sos_lemmas : list expr) : tactic unit := with_trim $ do
+meta structure super.opts :=
+(max_iters : ℕ := 200)
+(timeout : ℕ := 20000)
+
+meta def super (sos_lemmas : list expr) (os : super.opts) : tactic unit := do
+try_for os.timeout $ with_trim $ do
 as_refutation, local_false ← target,
 clauses ← clauses_of_context,
 sos_clauses ← sos_lemmas.mmap (clause.of_proof local_false),
@@ -100,7 +107,7 @@ infs ← inf_names.mmap $ λn, eval_expr inf_decl (const n []),
 infs ← return $ list.map inf_decl.inf $ list.sort_on inf_decl.prio infs,
 res ← (run_prover_loop selection21 (age_weight_clause_selection 3 4)
   default_preprocessing infs
-  0).run initial_state,
+  os.max_iters 0).run initial_state,
 match res with
 | (some empty_clause, st) := apply empty_clause >> skip
 | (none, saturation) := do sat_fmt ← pp saturation,
@@ -122,11 +129,12 @@ n ← get_unused_name p.get_app_fn.const_name none,
 tactic.assertv n t p
 
 meta def super (extra_clause_names : parse $ many ident)
-               (extra_lemma_names : parse with_ident_list) : tactic unit := do
+               (extra_lemma_names : parse with_ident_list)
+               (opts : super.opts := {}) : tactic unit := do
 with_lemmas extra_clause_names,
 extra_lemmas ← extra_lemma_names.mmap (λ c, do
   eqn_ls ← get_eqn_lemmas_for tt c,
   (c::eqn_ls).mmap mk_const),
-_root_.super extra_lemmas.join
+_root_.super extra_lemmas.join opts
 
 end tactic.interactive
